ToCoq.v
@@ -176,17 +176,17 @@ Proof.
 Qed.
 
 Lemma interp_term_closed genv lenv t :
- closed t = true ->
+ closed t ->
  interp_term genv lenv t = interp_term genv [] t.
 Proof.
- unfold closed. rewrite eqb_eq. intros E.
- apply (interp_term_more_lenv genv [] lenv). simpl. omega.
+ unfold closed. intros E.
+ apply (interp_term_more_lenv genv [] lenv). simpl. auto with *.
 Qed.
 
 Lemma interp_term_bsubst genv lenv u m n t :
  (level t <= S n)%nat ->
  List.length lenv = n ->
- closed u = true ->
+ closed u ->
  interp_term genv [] u = m ->
  interp_term genv (lenv++[m]) t =
   interp_term genv lenv (bsubst n u t).
@@ -209,7 +209,7 @@ Qed.
 Lemma interp_form_bsubst genv lenv u m n f :
  (level f <= S n)%nat ->
  List.length lenv = n ->
- closed u = true ->
+ closed u ->
  interp_term genv [] u = m ->
  interp_form genv (lenv++[m]) f <-> interp_form genv lenv (bsubst n u f).
 Proof.
@@ -238,12 +238,14 @@ Qed.
 
 Lemma interp_form_bsubst0 genv u m f :
  (level f <= 1)%nat ->
- closed u = true ->
+ closed u ->
  interp_term genv [] u = m ->
  interp_form genv [m] f <-> interp_form genv [] (bsubst 0 u f).
 Proof.
  intros. apply (@interp_form_bsubst genv [] u m 0 f); auto.
 Qed.
+
+Ltac prove_ext := intros ? ?; cbn; case eqbspec; auto; varsdec.
 
 Lemma interp_form_bsubst_adhoc genv m x f :
  (level f <= 1)%nat ->
@@ -254,10 +256,18 @@ Lemma interp_form_bsubst_adhoc genv m x f :
 Proof.
  intros.
  rewrite <- interp_form_bsubst0 with (m:=m); auto.
- - apply interp_form_ext. intros v Hv.
-   case eqbspec; auto. intros ->. varsdec.
+ - apply interp_form_ext. prove_ext.
  - cbn. now rewrite eqb_refl.
 Qed.
+
+Lemma interp_ctx_cons genv f c :
+ interp_form genv [] f ->
+ interp_ctx genv [] c ->
+ interp_ctx genv [] (f::c).
+Proof.
+ intros Hf Hc f' [<-|Hf']; auto.
+Qed.
+Hint Resolve interp_ctx_cons.
 
 Definition CoqRequirements lg :=
  match lg with
@@ -273,86 +283,68 @@ Definition CoqRequirements lg :=
     the proof, as in [Pred("=",[])->Pred("=",[])], and we'll
     end up with uninteresting (but true) evaluations. *)
 
-Lemma correctness :
- forall (d:derivation) logic genv,
+Ltac instlevel :=
+ repeat match goal with
+ | H : level ?d = 0 -> _ |- _ =>
+   let LV := fresh "LV" in
+   assert (LV : level d = 0) by intuition;
+   specialize (H LV)
+ end.
+
+Ltac tryinstgenv :=
+ repeat match goal with
+ | H : (forall (genv:variable->M), _), genv: variable->M |- _ =>
+   specialize (H genv)
+ end.
+
+Ltac substClaim :=
+ repeat match goal with
+ | H : Claim _ _ |- _ => red in H; rewrite H in * end.
+
+Lemma correctness (logic:Mix.logic)(d:derivation) :
  CoqRequirements logic ->
- closed d = true ->
- valid_deriv logic d = true ->
- interp_seq genv [] (dseq d).
+ Valid logic d ->
+ closed d ->
+ forall genv, interp_seq genv [] (claim d).
 Proof.
- induction d as [r s ds IH] using derivation_ind'.
- cbn - [valid_deriv_step].
- intros logic genv.
- rewrite !lazy_andb_iff. rewrite eqb_eq, !max_0.
- intros CR (Lr&Ls&Lds) (V,Vds).
- assert (IH' : Forall (fun d => forall genv, interp_seq genv [] (dseq d)) ds).
- { rewrite Forall_forall, forallb_forall in *.
-   rewrite list_max_0 in Lds.
-   intros d Hd genv'. eapply IH; eauto.
-   unfold closed. rewrite eqb_eq. apply Lds. now apply in_map. }
- clear IH Vds. cbn in *. break; mytac; cbn in *; intros Hc.
- - now apply Hc, list_mem_in.
- - destruct (H genv); auto.
- - intro Hf. apply (H genv).
-   intros ? [<-|E]; auto.
- - apply (H4 genv); auto.
- - intuition.
- - apply (H genv); auto.
- - apply (H genv); auto.
- - intuition.
- - intuition.
- - destruct (H2 genv); auto.
-   + apply (H4 genv). intros ? [<-|E]; auto.
-   + apply (H3 genv). intros ? [<-|E]; auto.
- - intros Hf1. apply (H genv). intros ? [<-|E]; auto.
- - apply (H1 genv); auto.
+ unfold closed.
+ intros CR.
+ induction 1; intros CL genv Hc; substClaim;
+  cbn in CL; rewrite ?eqb_eq, ?max_0 in CL;
+  instlevel; cbn in *; try (tryinstgenv; intuition eauto 3; fail).
  - intros m.
-   rewrite <- not_false_iff_true, negb_false_iff in H0.
-   rewrite Vars.mem_spec in H0.
-   rewrite interp_form_bsubst_adhoc with (x:=v).
-   apply H2.
-   rewrite <- (interp_ctx_ext genv); auto.
-   intros y Hy. case eqbspec; auto. intros <-. varsdec.
-   omega with *.
-   varsdec.
- - rewrite <- interp_form_bsubst0 with (u:=wit); auto.
-   rewrite !max_0 in Lds. intuition.
-   unfold closed. rewrite eqb_eq. intuition.
- - exists (interp_term genv [] wit).
-   rewrite interp_form_bsubst0 with (u:=wit); auto.
-   rewrite !max_0 in Ls. intuition.
-   unfold closed. rewrite eqb_eq. intuition.
- - destruct (H3 genv) as (m & Hm); auto.
-   rewrite <- not_false_iff_true, negb_false_iff in H0.
-   rewrite Vars.mem_spec in H0.
-   rewrite interp_form_bsubst_adhoc with (x:=v) in Hm.
+   rewrite interp_form_bsubst_adhoc with (x:=x) by auto with *.
+   apply IHValid.
+   rewrite <- (interp_ctx_ext genv); auto with *.
+ - rewrite <- interp_form_bsubst0 with (u:=t); auto with *.
+   destruct d as (?,s,?); cbn in *; subst s; cbn in *; omega with *.
+ - exists (interp_term genv [] t).
+   rewrite interp_form_bsubst0 with (u:=t); auto with *.
+ - destruct (IHValid1 genv) as (m & Hm); auto.
+   rewrite interp_form_bsubst_adhoc with (x:=x) in Hm; [ | | varsdec].
    erewrite interp_form_ext.
-   eapply H5.
-   intros A [<-|HA]. eapply Hm.
-   rewrite <- (interp_form_ext genv); auto.
-   intros y Hy. case eqbspec; auto. intros ->.
-   assert (Vars.In v (fvars c)).
-   { unfold fvars, fvars_list. rewrite vars_unionmap_in.
-     exists A; now split. }
-   varsdec.
-   intros y Hy. cbn. case eqbspec; auto. intros ->. varsdec.
-   rewrite !max_0 in Lds. intuition.
-   varsdec.
- - destruct (CR (interp_form genv [] f0)); auto.
-   destruct (H genv). intros A [<-|HA]; auto.
+   eapply IHValid2; eauto.
+   apply interp_ctx_cons. apply Hm.
+   now rewrite <- (interp_ctx_ext genv) by prove_ext.
+   prove_ext.
+   destruct d1 as (?,s,?); cbn in *; subst s; cbn in *; omega with *.
+ - subst logic.
+   destruct (CR (interp_form genv [] A)); auto.
+   destruct (IHValid genv); auto.
 Qed.
 
 (** We hence cannot have a valid proof of False in an empty context. *)
 
 Lemma coherence logic : CoqRequirements logic ->
  forall (d:derivation),
- closed d = true ->
- valid_deriv logic d = true ->
- dseq d <> ([]⊢False)%form.
+ Valid logic d ->
+ closed d ->
+ ~Claim d ([]⊢False).
 Proof.
- intros CR d CL VD E.
+ intros CR d VD CL E.
+ red in E.
  set (genv := fun (_:variable) => Mo.(someone)).
- assert (interp_seq genv [] (dseq d)).
+ assert (interp_seq genv [] (claim d)).
  { apply correctness with logic; auto. }
  rewrite E in H. cbn in *. apply H. intros A. destruct 1.
 Qed.
